\documentclass{article}
\usepackage[utf8]{inputenc}
\usepackage[margin=1in]{geometry}
\usepackage{amsmath, amsfonts, amsthm}
\usepackage{fancyhdr}
\usepackage{multicol}
\usepackage{graphicx}
\usepackage[inline]{enumitem}
\usepackage{wrapfig}
\usepackage[export]{adjustbox}
\graphicspath{ {images/} }
\pagestyle{empty}
\fancyhf{}
\cfoot{\thepage}
\pagenumbering{gobble}

\lhead{MATB42: Assignment \#9 \\
       Bonus}
\rhead{
Poon, Keegan\\
1002423727\\
Mar 27th 2018}
\newcommand{\norm}[1]{\| #1 \|}
\newcommand{\deriv}[1]{\frac{d}{d #1}}
\newcommand{\parti}[1]{\frac{\partial}{\partial #1}}
\renewcommand{\headrulewidth}{0pt}
\newcommand{\gam}{\boldsymbol{\gamma}}
\newcommand{\divt}{\text{div}}
\begin{document}

\thispagestyle{fancy}
\begin{enumerate}
    \item 
    \begin{enumerate}
        \item Let $f, g: \mathbb{R}^n \rightarrow \mathbb{R}; \; \boldsymbol F,\, \boldsymbol G :\; \mathbb{R}^n \rightarrow \mathbb{R}^n;$ and define $\Delta$, the \textit{Laplacian}, by $\displaystyle \Delta f = \sum_{i=1}^n \frac{\partial^2 f}{\partial x_i^2}$.

        Verify the following identities
        \begin{enumerate}[label=(\roman*)]
            \item div$ (\boldsymbol F + \boldsymbol G) =$ div $\boldsymbol F + $ div $\boldsymbol G$.
            \[ \divt( \boldsymbol F + \boldsymbol G) = \sum_{i=1}^n \frac{\partial (F_i + G_i)}{\partial x_i} = \sum_{i=1}^n \frac{\partial F_i}{\partial x_i} + \frac{\partial G_i}{\partial x_i} = \sum_{i=1}^n \frac{\partial F_i}{\partial x_i} + \sum_{i=1}^n \frac{\partial G_i}{\partial x_i} = \divt \boldsymbol F + \divt \boldsymbol G\]
            \item div$ (f \boldsymbol F ) =f$ div $\boldsymbol F + \boldsymbol F \cdot$ grad$f$.

            \[\divt (f \boldsymbol F) = \sum_{i=1}^n \frac{\partial fF_i}{\partial x_i} = \sum_{i=1}^n \frac{\partial f}{\partial x_i} F_i + \frac{\partial F_i}{\partial x_i}f = \sum_{i=1}^n \frac{\partial f}{\partial x_i} F_i + f \sum_{i=1}^n\frac{\partial F_i}{\partial x_i} = \nabla f \cdot \boldsymbol F + f \divt \boldsymbol F \]
            \item $\Delta (f g) =f \Delta g + g \Delta f + 2($grad$f)\cdot ( $grad$ g).$
            \begin{proof}
                \begin{align*}
                    \Delta(fg) &= \sum_{i=1}^n\frac{\partial^2fg}{\partial^2 x_i } \\
                    &= \sum_{i=1}^n\frac{\partial}{\partial x_i } \bigg[ \frac{\partial f}{\partial x_i }g  + \frac{\partial g}{\partial x_i }f\bigg] \\
                    &= \sum_{i=1}^n \bigg[ \frac{\partial f}{\partial^2 x_i }g  + \bigg( \frac{\partial f}{\partial x_i } \cdot \frac{\partial g}{\partial x_i } \bigg) + \frac{\partial g}{\partial^2 x_i }f + \bigg( \frac{\partial f}{\partial x_i } \cdot \frac{\partial g}{\partial x_i } \bigg)\bigg] \\
                    &= g\sum_{i=1}^n \frac{\partial f}{\partial^2 x_i }  + 2 \sum_{i=1}^n \bigg( \frac{\partial f}{\partial x_i } \cdot \frac{\partial g}{\partial x_i } \bigg) + f\sum_{i=1}^n \frac{\partial g}{\partial^2 x_i } \\
                    &= g \Delta f  + 2[\nabla f \cdot \nabla g] + f \Delta g\\
                \end{align*}
            \end{proof}
        \end{enumerate}
        \item Let $f,g:D \subset \mathbb{R}^3 \rightarrow \mathbb{R}$ be of class $C^1$. If $R$ is a solid region contained in $D$ then
        \[\iiint_R \nabla f \cdot \nabla g \, dV = \iint_{\partial R} f \nabla  g \cdot \boldsymbol n \, dS - \iiint_R f \nabla^2 g \, dV\] 
        $(\nabla^2 g = $ div $(\nabla g))$.

        \begin{proof}
            \begin{align*}
                \iiint_R \nabla f \cdot \nabla g \, dV = \iint_{\partial R} f \nabla  g \cdot \boldsymbol n \, dS - \iiint_R f \nabla^2 g \, dV \\
               \iff \iiint_R \nabla f \cdot \nabla g \, dV + \iiint_R f \nabla^2 g \, dV = \iint_{\partial R} f \nabla  g \cdot \boldsymbol n \, dS \\
            \end{align*}
            \begin{align*}
                \iint_{\partial R} f \nabla  g \cdot \boldsymbol n \, dS \overset{\text{Div Thm}}{=} \iiint_R \text{div} (f \nabla g) \, dV  \overset{\text{(ii)}}{=} \iiint_R f(\text{div} \nabla g) + \nabla g \cdot \nabla f \, dV  \\
                = \iiint_R f(\text{div} \nabla g) \, dV + \iiint_R \nabla f \cdot \nabla g \, dV = \iiint_R f \nabla^2 g \, dV + \iiint_R \nabla f \cdot \nabla g \, dV \\
            \end{align*}
        \end{proof}
    \end{enumerate} 
    \newpage
    \item Use the Divergence Theorem to verify your answer to question 7 on assignment 8.

    Let $S$ be the closed surface that consists of the hemisphere $x^2+y^2+z^2 = 1,\, z \geq 0,$ and its base $x^2 + y^2 \leq 1,\, z = 0.$ let $\boldsymbol E$ be the electric field $\boldsymbol E(x,y,z) = (2x,2y,2z)$. Calculate the electric flux across $S$ using Divergence Theorem.

    Divergence Theorem gives that 
    \[\iiint_R \divt \boldsymbol F \, dV = \iint_S \boldsymbol F \cdot d\boldsymbol S\]

    $S$ is a closed surface, and assuming the default outward normal Divergence Theorem. To integrate over the region, switch to polars restricting $\varphi \in [0,\pi/2]$ to restrict to the upper half. Together with $\divt \boldsymbol E = 6$ gives:
        \[ \iint_S \boldsymbol E \cdot d\boldsymbol S = \int_0^1 \int_0^{2\pi} \int_0^{\frac{\pi}{2}} 6 \rho^2 \sin \varphi \, d\varphi \, d\theta \, d\rho  = 12 \pi \int_0^1 \rho^2 \big[ -\cos \varphi\big]_0^{\frac{\pi}{2}} \, d\rho = 12\pi\bigg[\frac{\rho^3}{3} \bigg]_0^1 = 4\pi \]

    \item Let $\boldsymbol F (x,y,z) = (x,y^2,e^{yz})$ and let $R$ be a cube centered at the origin with sides of length 2. Evaluate $\displaystyle \int_S$ div $\boldsymbol F \, dV $ directly and by using the Divergence Theorem. 

    Directly:
    \begin{multicols}{2}
    \noindent 
    \begin{align*}
        \int_S \divt \boldsymbol F \, dV &= \int_{-1}^1 \int_{-1}^1 \int_{-1}^1 1 + 2y + ye^{yz} \, dx \, dz \, dy \\
        &= \int_{-1}^1 \int_{-1}^1 2 + 4y + 2ye^{yz} \, dz \, dy \\
    \end{align*}
    \begin{align*}
        &= \int_{-1}^1 4 + 8y + \big[e^{yz}\big]_{-1}^1\, dy \\
        &= \int_{-1}^1 4 + 8y + e^y - e^{-y} \, dy \\
        &= 8 + 0 + [e^y]_{-1}^1 + [e^{-y}]_{-1}^1 = 8
    \end{align*}
    \end{multicols} 
    Divergence:
        \[\int_R \divt \boldsymbol F \, dV = \int_S \boldsymbol F \cdot d\boldsymbol S\]
        where $S$ is the union of 6 planes with $-1 \leq x,y,z \leq 1$ and having normals in the $\pm x,y,z$ directions.
        The parameterizations can be given by
        \begin{align*}
            \boldsymbol \Phi_{S_1} (x,y) &= (x,y,1)\; &\boldsymbol \Phi_{S_1'} (x,y) &= (x,y,-1)\\
            \boldsymbol \Phi_{S_2} (y,z) &= (1,y,z)\; &\boldsymbol \Phi_{S_2'} (y,z) &= (-1,y,z)\\
            \boldsymbol \Phi_{S_3} (x,z) &= (x,1,z)\; &\boldsymbol \Phi_{S_3'} (x,z) &= (x,-1,z)\\
        \end{align*}
        When plugging in $S_3,S_3'$ into $\boldsymbol F$, then taking the dot with the normal, we get that the integrands are going to be the same, specifically 1. When doing the same with $S_2,S_2$, due to $x$ being odd, we get both being negative the other, so integrating over the same range will cancel each other out. Putting this together, the integral over $S$ is:
        \begin{align*}
            \int_S \boldsymbol F \cdot d\boldsymbol S &= 2 \int_{-1}^{1} \int_{-1}^{1} 1 \, dx \, dz + \int_{-1}^{1} \int_{-1}^{1} e^y \, dx \, dy + \int_{-1}^{1}\int_{-1}^{1} - e^{-y} \,dx\, dy \\
            &= 8 + 2\int_{-1}^{1} e^y \, dy - 2 \int_{-1}^{1} e^{-y} \, dy \\
            &= 8 + 2([e^y]_{-1}^1 + [e^{-y}]_{-1}^1) = 8
        \end{align*}
        \newpage
        \item Let $B$ be the pyramid with top vertex (0,0,1) and base vertices (0,0,0), (1,0,0), (0,1,0) and (1,1,0). Let $S$ be the 2-dim closed surface bounding $B$, oriented in the outward direction. Use Gauss' theorem to calculate $\displaystyle \int_S \boldsymbol F \cdot \, d \boldsymbol S$, where $\boldsymbol F(x,y,z) = (x^2y,3y^2z,9z^2x).$
            \[\iiint_R \divt \boldsymbol F \, dV = \iint_S \boldsymbol F \cdot d\boldsymbol S\]
            \begin{align*}
                \divt \boldsymbol F &= 2xy + 6yz + 18zx \\
                \iiint_R \divt \boldsymbol F \, dV &= \int_0^1 \int_0^{1-z} \int_0^{1-z} 2xy + 6yz + 18zx \, dx \, dy \, dz \\
                &= \int_0^1 \int_0^{1-z} (1-z)^2y + 6yz(1-z) + 9z(1-z)^2 \, dy \, dz \\
                &= \int_0^1 (1/2)(1-z)^4 + 3z(1-z)^3 + 9z(1-z)^3 \, dz \\
                &= \int_0^1 -\frac{23z^4}{2} + 34z^3 - 33z^2 + 10z + \frac{1}{2} \, dz \\
                &= -\frac{23}{10} + \frac{34}{4} - 11 + 5 + \frac{1}{2} \\
                &= \frac{7}{10} \\ 
            \end{align*}
            \newpage
\item Use the Divergence Theorem to evaluate $\displaystyle \int_S \boldsymbol F \cdot \, d \boldsymbol S,$ where $\displaystyle \boldsymbol F (x,y,z) = \bigg(z^2 x, \frac{y^3}{3} + \tan z, x^2z+y^2 \bigg)$ and $S$ is the top half of the unit sphere $x^2 + y^2 + z^2 = 1$, oriented by the unit normal which points away from the origin.
    
    For the Divergence Theorem to apply, the integral must be over a closed, oriented outwards. To use Divergence Theorem the surface needs to be closed, so add the disk $S'$ on the $xy$-plane to the surface. Then
    \[\iiint_R \divt \boldsymbol F \, dV - \iint_{S'} \boldsymbol F \cdot d \boldsymbol S = \iint_S \boldsymbol F \cdot d\boldsymbol S\]
    The disk can be parametrized as $\boldsymbol \Phi (r, \theta) = (r\cos \theta, r\sin \theta, 0)$ with $r \in [0,1], \theta \in [0,2\pi]$ The normal, pointing outward needs to be downward.
    \begin{align*} 
        \iint_{S'} \boldsymbol F \cdot d \boldsymbol S &= \int_0^1 \int_0^{2\pi} (*,*,(r\sin \theta)^2) \cdot (0,0,-1) \, d \theta \,d r \\
        &= - \int_0^1 \int_0^{2\pi} (r\sin \theta)^2 \, d \theta \,d r \\
        &= - \int_0^1 \int_0^{2\pi} r^2 (1/2 - (\cos \theta)/2) \, d \theta \,d r \\
        &= - \int_0^1 \pi r^2 \,d r = - \frac{\pi}{3}
    \end{align*}
    Meanwhile, the region enclosed by this, is the top half of the unit sphere, so switch to polars, restricting $\varphi \in [0,\pi/2]$ to remain above the $xy$-plane.
    \[\divt \boldsymbol F = z^2 + y^2 + x^2 = \rho\]
    \begin{align*} 
        \iiint_R \divt \boldsymbol F \, dV &= \int_0^1 \int_0^{2\pi} \int_0^{\frac{\pi}{2}} \rho^3 \sin\varphi \, d\varphi \, d\theta \, d \rho \\
        &= 2\pi \int_0^1 \rho^3 \big[ -\cos\varphi\big]_0^{\frac{\pi}{2}} \, d \rho = \frac{\pi}{2} \\
        & \implies \iint_S \boldsymbol F \cdot d \boldsymbol S = \frac{\pi}{2} + \frac{\pi}{3} = \frac{5\pi}{6}
    \end{align*}


\newpage
\item Let the electric field from a point source at the origin be given by $\displaystyle \boldsymbol E (\boldsymbol x) = \frac{\boldsymbol x}{\norm{\boldsymbol x}^3}$
    \begin{enumerate}
        \item What is the outward flux of $\boldsymbol E$ across the surface $\displaystyle \frac{x^2}{3} + \frac{2y^2}{5} + z^2 = 7$. 
            
            The surface is an ellipsoid centered around the origin. Since $\boldsymbol E$ follows the formula for Gauss' Law and the ellipsoid is closed and bounded, the flux of the surface is just $4\pi$.

        \item Show that the flux of $\boldsymbol E$ across that part of the sphere $x^2 + y^2 + z^2 = 25$ with $z \geq 3$ is equal to the flux across that part of the plane $z = 3$ with $x^2 + y^2 \leq 16$.
            
            \begin{proof}
            First, examining the sphere, closing it with the disk at $z=3$ allows the Divergence Theorem to be applied, but that is exactly the other surface given. Label the union of the two surfaces $S$. Since both the hemisphere and plane are above the $xy$-plane, $\boldsymbol 0 \not \in S$, and since $\boldsymbol E$ satifies inverse square we have that the flux of the surface $S$ is 0 by Gauss'. Now applying divergence, since $S$ is closed and bounded, we have that the sum of the flux of the hemisphere $S_1$ and the plane $S_2$ is 0. Looking symbolically, we have
                    \[\int_{S_1} \boldsymbol E \cdot \boldsymbol n_1 \, dS_1 = - \int_{S_2} \boldsymbol E \cdot \boldsymbol n_2 \, dS_2 \]
                But now they are oriented in opposite direction since the outward normal of $S$ has the normal of $S_1$ pointing away from the origin, and vice versa for $S_2$. If we reorient $S_2$ in the same direction, (with $-\boldsymbol n_2$) we get:
                    \[\int_{S_1} \boldsymbol E \cdot \boldsymbol n_1 \, dS_1 = \int_{S_2} \boldsymbol E \cdot \boldsymbol n_2 \, dS_2 \]
                    So the flux of both surfaces is the same.
            \end{proof}

    \end{enumerate} 
\newpage
\item Let $f : \mathbb{R}^n \rightarrow \mathbb{R}$ be given by $f(x,y,z) = x^2yz$ and let $\eta$ be the 2-form on $\mathbb{R}^3$ given by \[ \eta = (\sin x) \, dx \, dy + (e^y + xyz) \, dx \, dz + (x^2y^2) \, dy \, dz .\]
    \begin{enumerate}
        \item Compute $df$ and $d\eta$.

            $f$ is a 0 form so  $\displaystyle df = \sum_{i=0}^n \parti{x_i}f\, dx_i \implies df = 2xyz \, dx + x^2z \, dy + x^2y \, dz$
            \begin{align*} 
                d\eta &= d(\sin x) \wedge dx \wedge dy + d(e^y + xyz) \wedge dx \wedge dz + d(x^2y^2) \wedge dy \wedge dz \\
                &= (\cos x \, dx + 0 \, dy + 0 \, dz) \wedge dx \wedge dy + (yz \, dx + e^y + xz \, dy + xy \, dz) \wedge dx \wedge dz + d(x^2y^2) \wedge dy \wedge dz \\
                &=  (yz \, dx + e^y + xz \, dy + xy \, dz) \wedge dx \wedge dz + d(x^2y^2) \wedge dy \wedge dz \\
                &=  (yz \, dx + e^y + xz \, dy + xy \, dz) \wedge dx \wedge dz + (2xy^2 \, dx + 2x^2y \, dy) \wedge dy \wedge dz \\
                &= (e^y + xz) \, dy \wedge dx \wedge dz + (2xy^2) \, dx \wedge dy \wedge dz \\
                &= -(e^y + xz) \, dx \wedge dy \wedge dz + (2xy^2) \, dx \wedge dy \wedge dz \\
                &= (2xy^2 - e^y + xz) \, dx \wedge dy \wedge dz \\
            \end{align*} 
        \item Evaluate $df \wedge \eta$.
            \begin{align*} 
                & (2xyz \, dx + x^2z \, dy + x^2y \, dz) \wedge ((\sin x) \, dx \, dy + (e^y + xyz) \, dx \, dz) \\
                &= (2xyz) \, dx \wedge ((\sin x) \, dx \, dy + (e^y + xyz) \, dx \, dz) \\
                & \; \; \; \; + (x^2z) \, dy \wedge ((\sin x) \, dx \, dy + (e^y + xyz) \, dx \, dz) \\
                & \; \; \; \; + (x^2y) \, dz \wedge ((\sin x) \, dx \, dy + (e^y + xyz) \, dx \, dz) \\
                & = (x^2z) \, dy \wedge ((e^y + xyz) \, dx \, dz) + (x^2y) \, dz \wedge ((\sin x) \, dx \, dy) \\
                & = ((x^2z)(e^y + xyz) \, dy \, dx \, dz) + ((x^2y) (\sin x) \, dz \, dx \, dy) \\
                & = -((x^2z)(e^y + xyz) \, dx \, dy \, dz) + ((x^2y) (\sin x) \, dx \, dy \, dz ) \\
                & = ((x^2y)(\sin x) - (x^2z)(e^y + xyz)) \, dx \, dy \, dz \\
                & = x^2(y\sin x - ze^y - xyz^2) \, dx \, dy \, dz \\
            \end{align*} 

    \end{enumerate} 
\end{enumerate}
\newpage
\section*{Bonus}
Use Gauss' Divergence Theorem to evaluate $\boldsymbol F = (x^3, 0, z^3)$ over the surface $S$, where $S$ is the upper hemisphere of $x^2 + y^2 + z^2 = 4$.
    
    For the Divergence Theorem to apply, the surface needs to be closed, so add the disk at $z = 0$ to enclose the upper hemisphere. Now the theorem applies for $S' = S \cup S_{D}$ (where $S_D$ is the disk) and gives that
    \[ \iiint_R \divt \boldsymbol F \, dV = \iint_S \boldsymbol F \cdot d \boldsymbol S + \iint_{S_D} \boldsymbol F \cdot d \boldsymbol S \]
    \[ \iff \iiint_R \divt \boldsymbol F \, dV - \iint_{S_D} \boldsymbol F \cdot d \boldsymbol S = \iint_S \boldsymbol F \cdot d \boldsymbol S \]
    Evaluate $\displaystyle \iiint_R \divt \boldsymbol F \, dV$ using spherical polars, restricting $\varphi \in [0, \pi/2]$ to restrict to upper hemisphere, and the other variables the default limits for a sphere.
    \begin{align*} 
        \iiint_R \divt \boldsymbol F \, dV &= \int_0^{2} \int_0^{2\pi} \int_0^{\frac{\pi}{2}} (3(\rho \cos \theta \sin \varphi)^2 + 3(\rho \cos \varphi)^2 ) \rho^2 \sin \varphi \, d\varphi \, d\theta \, d\rho \\
        &= \int_0^{2} \int_0^{2\pi} \int_0^{\frac{\pi}{2}} 3\rho^2 (\cos^2 \theta \sin^2 \varphi + \cos^2 \varphi)\rho^2 \sin \varphi \, d\varphi \, d\theta \, d\rho \\
        &= \int_0^{2} \int_0^{2\pi} \int_0^{\frac{\pi}{2}} 3\rho^4 ((1 - \sin^2 \theta) \sin^2 \varphi + \cos^2 \varphi) \sin \varphi \, d\varphi \, d\theta \, d\rho \\
        &= \int_0^{2} \int_0^{2\pi} \int_0^{\frac{\pi}{2}} 3\rho^4 (\sin^2 \varphi + \cos^2 \varphi  - \sin^2 \theta \sin^2 \varphi ) \sin \varphi \, d\varphi \, d\theta \, d\rho \\
        &= \int_0^{2} \int_0^{2\pi} \int_0^{\frac{\pi}{2}} 3\rho^4 (1 - \sin^2 \theta (1 - \cos^2 \varphi)) \sin \varphi \, d\varphi \, d\theta \, d\rho \\
    \end{align*} 
    \begin{multicols}{2}
    \begin{align*} 
        &\; \; \; \; \text{Let } u = \cos \varphi ,\, du = -\sin \varphi \\
        &= \int_0^{2} \int_0^{2\pi} \int_1^0 -3\rho^4 (1 - \sin^2 \theta (1 - u)) \, du \, d\theta \, d\rho \\
        &= \int_0^{2} \int_0^{2\pi} \int_1^0 -3\rho^4 (1 - \sin^2 \theta + u^2\sin^2 \theta ) \, du \, d\theta \, d\rho \\
        &= \int_0^{2} \int_0^{2\pi} -3\rho^4 \bigg[u - u\sin^2 \theta + \frac{1}{3}u^3\sin^2 \theta \bigg]_1^0 \, d\theta \, d\rho \\
        &= \int_0^{2} \int_0^{2\pi} -3\rho^4 (-1 +\sin^2 \theta - \frac{1}{3}\sin^2 \theta) \, d\theta \, d\rho \\
    \end{align*} 
    \begin{align*} 
        &= \int_0^{2} \int_0^{2\pi} 3\rho^4 \bigg(1 - \frac{1 - \cos(2\theta)}{3}\bigg) \, d\theta \, d\rho \\
        &= \int_0^{2} \int_0^{2\pi} 3\rho^4 \bigg(\frac{2}{3} + \frac{\cos(2\theta)}{3}\bigg) \, d\theta \, d\rho \\
        &= \int_0^{2} \bigg[ 3\rho^4 \bigg(\frac{2}{3} \bigg) \theta \bigg]_0^{2\pi} \, d\rho \\
        &= \int_0^{2} \rho^4(4\pi) \, d\rho \\
        &= \bigg[\frac{4\rho^5\pi}{5} \bigg]_0^{2} = \frac{128\pi}{5}
    \end{align*}  
    \end{multicols}
    Evaluate $\displaystyle \iint_{S_D} \boldsymbol F \cdot d \boldsymbol S$ using parametrization of $\boldsymbol \Phi (\theta, r) = (r\cos \theta, r\sin \theta, 0),\, r\in [0, 2], \theta \in [0,2\pi]$, with downward normal to point outward from upper hemispher. 
   \[\iint_{S_D} \boldsymbol F \cdot d \boldsymbol S = \iint_{S_D} (*,*,0) \cdot (0,0,-1) \, dS = 0\]
   \[ \implies \iint_S \boldsymbol F \cdot d \boldsymbol S = \frac{128\pi}{5} \]
\end{document}
